Revised extension of Lib.IntTypes to signed integers
- Replaced `Lib.IntTypes.pow2_values` with these 3 specific instances

```FStar
val pow2_2: unit -> Lemma (pow2 2 = 4) [SMTPat (pow2 2)]
val pow2_3: unit -> Lemma (pow2 3 = 8) [SMTPat (pow2 3)]
val pow2_4: unit -> Lemma (pow2 4 = 16) [SMTPat (pow2 4)]
```

The rest follows from `FStar.UInt.LibIntTypes` which is in scope of
every module depending on `Lib.IntTypes`.

- Did a general cleanup on qualifiers
 - `inline_for_extraction unfold` is equivalent to just `unfold`
 - Many specification-level definitions and lemmas were marked `inline_for_extraction`
 - Some definitions where marked `inline_for_extraction` but they should have
   been marked as `unfold` to trigger patterns in lemmas. For instance,
   `uint_v`, `sint_v`, `uint`, and `sint` must be marked unfold in
   order to trigger the pattern in the `intv_injective lemma`. Same for
   `u1`, `u8`, etc.
 - Marking definitions as unfold also helps get rid off overly specific lemmas
   (e.g. `size_v_size_lemma`) that are instances of more general lemmas.

- Removed some unnecessary definitions
 - `nat_to_uint` is equivalent to `nat_to_int`, which is equivalent to `mk_int`.
 - `zero` and `one`, which can just be replaced by `0` and `1` in the contexts
   where they appeared.

- Added missing specifications for `neq_mask`, `lt_mask, `gt_mask`, `lte_mask`.

- Style cleanup
  - Removed unnecessary `requires`, `ensures`
  - Removed some implicit parameters passed explicitly which just obscure
    lemma statements.

lib/Lib.IntTypes.fst
@@ -1,53 +1,18 @@
 module Lib.IntTypes
 
-(* Declared in .fsti : intsize, bits, maxint *)
-#set-options "--z3rlimit 50 --max_fuel 0 --max_ifuel 1"
+open FStar.Math.Lemmas
 
-let pow2_values n =
-    assert_norm (pow2 0 = 1);
-    assert_norm (pow2 1 = 2);
-    assert_norm (pow2 2 = 4);
-    assert_norm (pow2 3 = 8);
-    assert_norm (pow2 4 = 16);
-    assert_norm (pow2 8 = 0x100);
-    assert_norm (pow2 16 = 0x10000);
-    assert_norm (pow2 32 = 0x100000000);
-    assert_norm (pow2 64 = 0x10000000000000000);
-    assert_norm (pow2 128 = 0x100000000000000000000000000000000)
+#push-options "--max_fuel 0 --max_ifuel 1 --z3rlimit 50"
+
+let pow2_2 _ = assert_norm (pow2 2 = 4)
+let pow2_3 _ = assert_norm (pow2 3 = 8)
+let pow2_4 _ = assert_norm (pow2 4 = 16)
 
 let sec_int_t t = pub_int_t t
 
 let sec_int_v #t u = pub_int_v u
 
-val intv_extensionality:
-   #t:inttype
- -> #l:secrecy_level
- -> a:int_t t l
- -> b:int_t t l
- -> Lemma
-  (requires int_v #t #l a == int_v #t #l b)
-  (ensures  a == b)
-  
-let intv_extensionality #t #l a b =
-  match t with
-  | U1   -> ()
-  | U8   -> UInt8.v_inj a b
-  | U16  -> UInt16.v_inj a b
-  | U32  -> UInt32.v_inj a b
-  | U64  -> UInt64.v_inj a b
-  | U128 -> UInt128.v_inj a b
-  | S8   -> Int8.v_inj a b
-  | S16  -> Int16.v_inj a b
-  | S32  -> Int32.v_inj a b
-  | S64  -> Int64.v_inj a b
-  | S128 -> Int128.v_inj a b
-
-
-(* Declared in .fsti: uint8, uint16, uint32, uint64, uint128 *)
-
 let secret #t x = x
-
-#reset-options
 
 let mk_int #t #l x =
   match t with
@@ -62,21 +27,33 @@ let mk_int #t #l x =
   | S32 -> Int32.int_to_t x
   | S64 -> Int64.int_to_t x
   | S128 -> Int128.int_to_t x
-  
-  
-let intv_injective #t #l a =
-  intv_extensionality a (mk_int (int_v a))
 
-(*let u16_us x = x
-let u32_ul x = x
-let u64_uL x = x
-*)
+val v_extensionality:
+   #t:inttype
+ -> #l:secrecy_level
+ -> a:int_t t l
+ -> b:int_t t l
+ -> Lemma
+  (requires v a == v b)
+  (ensures  a == b)
+let v_extensionality #t #l a b =
+  match t with
+  | U1   -> ()
+  | U8   -> UInt8.v_inj a b
+  | U16  -> UInt16.v_inj a b
+  | U32  -> UInt32.v_inj a b
+  | U64  -> UInt64.v_inj a b
+  | U128 -> UInt128.v_inj a b
+  | S8   -> Int8.v_inj a b
+  | S16  -> Int16.v_inj a b
+  | S32  -> Int32.v_inj a b
+  | S64  -> Int64.v_inj a b
+  | S128 -> Int128.v_inj a b
 
-//let u128 x = FStar.UInt128.uint64_to_uint128 (u64 x)
+let v_injective #t #l a =
+  v_extensionality a (mk_int (v a))
 
-let size_v_size_lemma s = ()
-
-let uint_v_size_lemma s = ()
+let v_mk_int #t #l n = ()
 
 let size_to_uint32 x = x
 
@@ -86,179 +63,183 @@ let byte_to_uint8 x = x
 
 let byte_to_int8 x = FStar.Int.Cast.uint8_to_int8 x
 
-let nat_to_int #t #l x =
-  match t with
-  | U1 -> u8 x
-  | U8 -> u8 x
-  | U16 -> u16 x
-  | U32 -> u32 x
-  | U64 -> u64 x
-  | U128 -> UInt128.uint_to_t x
-  | S8 -> i8 x
-  | S16 -> i16 x
-  | S32 -> i32 x
-  | S64 -> i64 x
-  | S128 -> Int128.int_to_t x
-  
-#reset-options "--z3rlimit 500"
+#push-options "--z3rlimit 200"
 
-let cast #t #l t' l' u  =
+let cast #t #l t' l' u =
+  assert_norm (pow2 8 = 2 * pow2 7); 
+  assert_norm (pow2 16 = 2 * pow2 15); 
+  assert_norm (pow2 128 = 2 * pow2 127); 
+  let open FStar.Int.Cast in
   match t, t' with
   | U1, U1 -> u
   | U1, U8 -> u
-  | U1, U16 -> FStar.Int.Cast.uint8_to_uint16 u
-  | U1, U32 -> FStar.Int.Cast.uint8_to_uint32 u
-  | U1, U64 -> FStar.Int.Cast.uint8_to_uint64 u
-  | U1, U128 -> FStar.UInt128.uint64_to_uint128 (FStar.Int.Cast.uint8_to_uint64 u)
-  | U1, S8 -> FStar.Int.Cast.uint8_to_int8 u
-  | U1, S16 -> FStar.Int.Cast.uint8_to_int16 u
-  | U1, S32 -> FStar.Int.Cast.uint8_to_int32 u
-  | U1, S64 -> FStar.Int.Cast.uint8_to_int64 u
-  | U1, S128 -> mk_int #S128 #l' (uint_v u)
-  | U8, U1 -> FStar.UInt8.rem u 2uy
+  | U1, U16 -> uint8_to_uint16 u
+  | U1, U32 -> uint8_to_uint32 u
+  | U1, U64 -> uint8_to_uint64 u
+  | U1, U128 -> UInt128.uint64_to_uint128 (uint8_to_uint64 u)
+  | U1, S8 -> uint8_to_int8 u
+  | U1, S16 -> uint8_to_int16 u
+  | U1, S32 -> uint8_to_int32 u
+  | U1, S64 -> uint8_to_int64 u
+  | U1, S128 -> pow2_le_compat (bits t' - 1) (bits t); mk_int #S128 #l' (v u)
+
+  | U8, U1 -> UInt8.rem u 2uy
   | U8, U8 -> u
-  | U8, U16 -> FStar.Int.Cast.uint8_to_uint16 u
-  | U8, U32 -> FStar.Int.Cast.uint8_to_uint32 u
-  | U8, U64 -> FStar.Int.Cast.uint8_to_uint64 u
-  | U8, U128 -> FStar.UInt128.uint64_to_uint128 (FStar.Int.Cast.uint8_to_uint64 u)
-  | U8, S8 -> FStar.Int.Cast.uint8_to_int8 u
-  | U8, S16 -> FStar.Int.Cast.uint8_to_int16 u
-  | U8, S32 -> FStar.Int.Cast.uint8_to_int32 u
-  | U8, S64 -> FStar.Int.Cast.uint8_to_int64 u
-  | U8, S128 -> pow2_le_compat ((bits t')-1) (bits t); mk_int #S128 #l' (uint_v u)
-  | U16, U1 -> FStar.Int.Cast.uint16_to_uint8 (FStar.UInt16.rem u 2us)
-  | U16, U8 -> FStar.Int.Cast.uint16_to_uint8 u
+  | U8, U16 -> uint8_to_uint16 u
+  | U8, U32 -> uint8_to_uint32 u
+  | U8, U64 -> uint8_to_uint64 u
+  | U8, U128 -> UInt128.uint64_to_uint128 (uint8_to_uint64 u)
+  | U8, S8 -> uint8_to_int8 u
+  | U8, S16 -> uint8_to_int16 u
+  | U8, S32 -> uint8_to_int32 u
+  | U8, S64 -> uint8_to_int64 u
+  | U8, S128 -> pow2_le_compat (bits t' - 1) (bits t); mk_int #S128 #l' (v u)
+
+  | U16, U1 -> uint16_to_uint8 (UInt16.rem u 2us)
+  | U16, U8 -> uint16_to_uint8 u
   | U16, U16 -> u
-  | U16, U32 -> FStar.Int.Cast.uint16_to_uint32 u
-  | U16, U64 -> FStar.Int.Cast.uint16_to_uint64 u
-  | U16, U128 -> FStar.UInt128.uint64_to_uint128 (FStar.Int.Cast.uint16_to_uint64 u)
-  | U16, S8 -> FStar.Int.Cast.uint16_to_int8 u
-  | U16, S16 -> FStar.Int.Cast.uint16_to_int16 u
-  | U16, S32 -> FStar.Int.Cast.uint16_to_int32 u
-  | U16, S64 -> FStar.Int.Cast.uint16_to_int64 u
-  | U16, S128 -> pow2_le_compat ((bits t')-1) (bits t); mk_int #S128 #l' (uint_v u)
-  | U32, U1 -> FStar.Int.Cast.uint32_to_uint8 (FStar.UInt32.rem u 2ul)
-  | U32, U8 -> FStar.Int.Cast.uint32_to_uint8 u
-  | U32, U16 -> FStar.Int.Cast.uint32_to_uint16 u
+  | U16, U32 -> uint16_to_uint32 u
+  | U16, U64 -> uint16_to_uint64 u
+  | U16, U128 -> UInt128.uint64_to_uint128 (uint16_to_uint64 u)
+  | U16, S8 -> uint16_to_int8 u
+  | U16, S16 -> uint16_to_int16 u
+  | U16, S32 -> uint16_to_int32 u
+  | U16, S64 -> uint16_to_int64 u
+  | U16, S128 -> pow2_le_compat (bits t' - 1) (bits t); mk_int #S128 #l' (v u)
+  
+  | U32, U1 -> uint32_to_uint8 (UInt32.rem u 2ul)
+  | U32, U8 -> uint32_to_uint8 u
+  | U32, U16 -> uint32_to_uint16 u
   | U32, U32 -> u
-  | U32, U64 -> FStar.Int.Cast.uint32_to_uint64 u
-  | U32, U128 -> FStar.UInt128.uint64_to_uint128 (FStar.Int.Cast.uint32_to_uint64 u)
-  | U32, S8 -> FStar.Int.Cast.uint32_to_int8 u
-  | U32, S16 -> FStar.Int.Cast.uint32_to_int16 u
-  | U32, S32 -> FStar.Int.Cast.uint32_to_int32 u
-  | U32, S64 -> FStar.Int.Cast.uint32_to_int64 u
-  | U32, S128 -> pow2_le_compat ((bits t')-1) (bits t); mk_int #S128 #l' (uint_v u)
-  | U64, U1 -> FStar.Int.Cast.uint64_to_uint8 (FStar.UInt64.rem u 2uL)
-  | U64, U8 -> FStar.Int.Cast.uint64_to_uint8 u
-  | U64, U16 -> FStar.Int.Cast.uint64_to_uint16 u
-  | U64, U32 -> FStar.Int.Cast.uint64_to_uint32 u
+  | U32, U64 -> uint32_to_uint64 u
+  | U32, U128 -> UInt128.uint64_to_uint128 (uint32_to_uint64 u)
+  | U32, S8 -> uint32_to_int8 u
+  | U32, S16 -> uint32_to_int16 u
+  | U32, S32 -> uint32_to_int32 u
+  | U32, S64 -> uint32_to_int64 u
+  | U32, S128 -> pow2_le_compat (bits t' - 1) (bits t); mk_int #S128 #l' (v u)
+  
+  | U64, U1 -> uint64_to_uint8 (UInt64.rem u 2uL)
+  | U64, U8 -> uint64_to_uint8 u
+  | U64, U16 -> uint64_to_uint16 u
+  | U64, U32 -> uint64_to_uint32 u
   | U64, U64 -> u
-  | U64, U128 -> FStar.UInt128.uint64_to_uint128 u
-  | U64, S8 -> FStar.Int.Cast.uint64_to_int8 u
-  | U64, S16 -> FStar.Int.Cast.uint64_to_int16 u
-  | U64, S32 -> FStar.Int.Cast.uint64_to_int32 u
-  | U64, S64 -> FStar.Int.Cast.uint64_to_int64 u
-  | U64, S128 -> pow2_le_compat ((bits t')-1) (bits t); mk_int #S128 #l' (uint_v u)
+  | U64, U128 -> UInt128.uint64_to_uint128 u
+  | U64, S8 -> uint64_to_int8 u
+  | U64, S16 -> uint64_to_int16 u
+  | U64, S32 -> uint64_to_int32 u
+  | U64, S64 -> uint64_to_int64 u
+  | U64, S128 -> pow2_le_compat (bits t' - 1) (bits t); mk_int #S128 #l' (v u)
+
   | U128, U1 ->
     assert_norm (pow2 64 * pow2 64 = pow2 128);
     assert_norm (pow2 8 * pow2 56 = pow2 64);
-    FStar.Math.Lemmas.modulo_modulo_lemma (uint_v u) (pow2 64) (pow2 64);
-    FStar.Math.Lemmas.modulo_modulo_lemma (uint_v u) (pow2 8) (pow2 56);
-    FStar.UInt8.rem (FStar.Int.Cast.uint64_to_uint8
-      (FStar.Int.Cast.Full.uint128_to_uint64 u)) 0x2uy
+    modulo_modulo_lemma (v u) (pow2 64) (pow2 64);
+    modulo_modulo_lemma (v u) (pow2 8) (pow2 56);
+    UInt8.rem (uint64_to_uint8 (FStar.Int.Cast.Full.uint128_to_uint64 u)) 0x2uy
   | U128, U8 ->
     assert_norm (pow2 64 * pow2 64 = pow2 128);
     assert_norm (pow2 8 * pow2 56 = pow2 64);
-    FStar.Math.Lemmas.modulo_modulo_lemma (uint_v u) (pow2 64) (pow2 64);
-    FStar.Math.Lemmas.modulo_modulo_lemma (uint_v u) (pow2 8) (pow2 56);
-    FStar.Int.Cast.uint64_to_uint8 (FStar.UInt128.uint128_to_uint64 u)
+    modulo_modulo_lemma (v u) (pow2 64) (pow2 64);
+    modulo_modulo_lemma (v u) (pow2 8) (pow2 56);
+    uint64_to_uint8 (UInt128.uint128_to_uint64 u)
   | U128, U16 ->
     assert_norm (pow2 64 * pow2 64 = pow2 128);
     assert_norm (pow2 16 * pow2 48 = pow2 64);
-    FStar.Math.Lemmas.modulo_modulo_lemma (uint_v u) (pow2 64) (pow2 64);
-    FStar.Math.Lemmas.modulo_modulo_lemma (uint_v u) (pow2 16) (pow2 48);
-    FStar.Int.Cast.uint64_to_uint16 (FStar.UInt128.uint128_to_uint64 u)
+    modulo_modulo_lemma (v u) (pow2 64) (pow2 64);
+    modulo_modulo_lemma (v u) (pow2 16) (pow2 48);
+    uint64_to_uint16 (UInt128.uint128_to_uint64 u)
   | U128, U32 ->
     assert_norm (pow2 64 * pow2 64 = pow2 128);
     assert_norm (pow2 32 * pow2 32 = pow2 64);
-    FStar.Math.Lemmas.modulo_modulo_lemma (uint_v u) (pow2 64) (pow2 64);
-    FStar.Math.Lemmas.modulo_modulo_lemma (uint_v u) (pow2 32) (pow2 32);
-    FStar.Int.Cast.uint64_to_uint32 (FStar.UInt128.uint128_to_uint64 u)
+    modulo_modulo_lemma (v u) (pow2 64) (pow2 64);
+    modulo_modulo_lemma (v u) (pow2 32) (pow2 32);
+    uint64_to_uint32 (UInt128.uint128_to_uint64 u)
   | U128, U64 ->
     assert_norm (pow2 64 * pow2 64 = pow2 128);
-    FStar.Math.Lemmas.modulo_modulo_lemma (uint_v u) (pow2 64) (pow2 64);
-    FStar.UInt128.uint128_to_uint64 u
+    modulo_modulo_lemma (v u) (pow2 64) (pow2 64);
+    UInt128.uint128_to_uint64 u
   | U128, U128 -> u
   | U128, S8 ->
     assert_norm (pow2 64 * pow2 64 = pow2 128);
     assert_norm (pow2 8 * pow2 56 = pow2 64);
-    FStar.Math.Lemmas.modulo_modulo_lemma (uint_v u) (pow2 64) (pow2 64);
-    FStar.Math.Lemmas.modulo_modulo_lemma (uint_v u) (pow2 8) (pow2 56);
-    FStar.Int.Cast.uint64_to_int8 (FStar.UInt128.uint128_to_uint64 u)
+    modulo_modulo_lemma (v u) (pow2 64) (pow2 64);
+    modulo_modulo_lemma (v u) (pow2 8) (pow2 56);
+    uint64_to_int8 (UInt128.uint128_to_uint64 u)
   | U128, S16 ->
     assert_norm (pow2 64 * pow2 64 = pow2 128);
     assert_norm (pow2 16 * pow2 48 = pow2 64);
-    FStar.Math.Lemmas.modulo_modulo_lemma (uint_v u) (pow2 64) (pow2 64);
-    FStar.Math.Lemmas.modulo_modulo_lemma (uint_v u) (pow2 16) (pow2 48);
-    FStar.Int.Cast.uint64_to_int16 (FStar.UInt128.uint128_to_uint64 u)
+    modulo_modulo_lemma (v u) (pow2 64) (pow2 64);
+    modulo_modulo_lemma (v u) (pow2 16) (pow2 48);
+    uint64_to_int16 (UInt128.uint128_to_uint64 u)
   | U128, S32 ->
     assert_norm (pow2 64 * pow2 64 = pow2 128);
     assert_norm (pow2 32 * pow2 32 = pow2 64);
-    FStar.Math.Lemmas.modulo_modulo_lemma (uint_v u) (pow2 64) (pow2 64);
-    FStar.Math.Lemmas.modulo_modulo_lemma (uint_v u) (pow2 32) (pow2 32);
-    FStar.Int.Cast.uint64_to_int32 (FStar.UInt128.uint128_to_uint64 u)
+    modulo_modulo_lemma (v u) (pow2 64) (pow2 64);
+    modulo_modulo_lemma (v u) (pow2 32) (pow2 32);
+    uint64_to_int32 (UInt128.uint128_to_uint64 u)
   | U128, S64 ->
     assert_norm (pow2 64 * pow2 64 = pow2 128);
-    FStar.Math.Lemmas.modulo_modulo_lemma (uint_v u) (pow2 64) (pow2 64);
-    FStar.Int.Cast.uint64_to_int64 (FStar.UInt128.uint128_to_uint64 u)  
-  | U128, S128 -> mk_int #S128 #l' (uint_v u @%. t')
-  | S8, U1 -> FStar.UInt8.rem (FStar.Int.Cast.int8_to_uint8 u) 2uy
-  | S8, U8 -> FStar.Int.Cast.int8_to_uint8 u
-  | S8, U16 -> FStar.Int.Cast.int8_to_uint16 u
-  | S8, U32 -> FStar.Int.Cast.int8_to_uint32 u
-  | S8, U64 -> FStar.Int.Cast.int8_to_uint64 u
-  | S8, U128 -> pow2_le_compat (bits t') ((bits t)-1); mk_int #U128 #l' (sint_v u % modulus U128)
-  | S8, S8 -> u
-  | S8, S16 -> FStar.Int.Cast.int8_to_int16 u
-  | S8, S32 -> FStar.Int.Cast.int8_to_int32 u
-  | S8, S64 -> FStar.Int.Cast.int8_to_int64 u
-  | S8, S128 ->  pow2_le_compat ((bits t')-1) ((bits t)-1); mk_int #S128 #l' (sint_v u)
-  | S16, U1 -> FStar.UInt8.rem (FStar.Int.Cast.int16_to_uint8 u) 2uy
-  | S16, U8 -> FStar.Int.Cast.int16_to_uint8 u
-  | S16, U16 -> FStar.Int.Cast.int16_to_uint16 u
-  | S16, U32 -> FStar.Int.Cast.int16_to_uint32 u
-  | S16, U64 -> FStar.Int.Cast.int16_to_uint64 u
-  | S16, U128 -> pow2_le_compat (bits t') ((bits t)-1); mk_int #U128 #l' (sint_v u % modulus U128)
-  | S16, S8 -> FStar.Int.Cast.int16_to_int8 u
+    modulo_modulo_lemma (v u) (pow2 64) (pow2 64);
+    uint64_to_int64 (UInt128.uint128_to_uint64 u)
+  | U128, S128 -> assert_norm (pow2 128 = 2 * pow2 127); mk_int #S128 #l' (v u @%. t')
+
+  | S8, U1 -> UInt8.rem (int8_to_uint8 u) 2uy
+  | S8, U8 -> int8_to_uint8 u
+  | S8, U16 -> int8_to_uint16 u
+  | S8, U32 -> int8_to_uint32 u
+  | S8, U64 -> int8_to_uint64 u
+  | S8, U128 -> pow2_le_compat (bits t') (bits t - 1); mk_int #U128 #l' (v u % modulus U128)
+  | S8, S8 ->  u
+  | S8, S16 -> int8_to_int16 u
+  | S8, S32 -> int8_to_int32 u
+  | S8, S64 -> int8_to_int64 u
+  | S8, S128 -> pow2_le_compat (bits t' - 1) (bits t - 1); mk_int #S128 #l' (v u)
+
+  | S16, U1 -> UInt8.rem (int16_to_uint8 u) 2uy
+  | S16, U8 -> int16_to_uint8 u
+  | S16, U16 -> int16_to_uint16 u
+  | S16, U32 -> int16_to_uint32 u
+  | S16, U64 -> int16_to_uint64 u
+  | S16, U128 -> pow2_le_compat (bits t') (bits t - 1); mk_int #U128 #l' (v u % modulus U128)
+  | S16, S8 -> int16_to_int8 u
   | S16, S16 -> u
-  | S16, S32 -> FStar.Int.Cast.int16_to_int32 u
-  | S16, S64 -> FStar.Int.Cast.int16_to_int64 u
-  | S16, S128 -> pow2_le_compat ((bits t')-1) ((bits t)-1); mk_int #S128 #l' (sint_v u)
-  | S32, U1 -> FStar.UInt8.rem (FStar.Int.Cast.int32_to_uint8 u) 2uy
-  | S32, U8 -> FStar.Int.Cast.int32_to_uint8 u
-  | S32, U16 -> FStar.Int.Cast.int32_to_uint16 u
-  | S32, U32 -> FStar.Int.Cast.int32_to_uint32 u
-  | S32, U64 -> FStar.Int.Cast.int32_to_uint64 u
-  | S32, U128 -> pow2_le_compat (bits t') ((bits t)-1); mk_int #U128 #l' (sint_v u % modulus U128)
-  | S32, S8 -> FStar.Int.Cast.int32_to_int8 u
-  | S32, S16 -> FStar.Int.Cast.int32_to_int16 u
-  | S32, S32 -> u
-  | S32, S64 -> FStar.Int.Cast.int32_to_int64 u
-  | S32, S128 -> pow2_le_compat ((bits t')-1) ((bits t)-1); mk_int #S128 #l' (sint_v u)
-  | S64, U1 -> FStar.UInt8.rem (FStar.Int.Cast.int64_to_uint8 u) 2uy
-  | S64, U8 -> FStar.Int.Cast.int64_to_uint8 u
-  | S64, U16 -> FStar.Int.Cast.int64_to_uint16 u
-  | S64, U32 -> FStar.Int.Cast.int64_to_uint32 u
-  | S64, U64 -> FStar.Int.Cast.int64_to_uint64 u
-  | S64, U128 -> pow2_le_compat (bits t') ((bits t)-1); mk_int #U128 #l' (sint_v u % modulus U128)
-  | S64, S8 -> FStar.Int.Cast.int64_to_int8 u
-  | S64, S16 -> FStar.Int.Cast.int64_to_int16 u
-  | S64, S32 -> FStar.Int.Cast.int64_to_int32 u
-  | S64, S64 -> u
-  | S64, S128 -> pow2_le_compat ((bits t')-1) ((bits t)-1); mk_int #S128 #l' (sint_v u)
-  | S128, S128 -> u
-  | S128, _ -> mk_int #t' #l' (sint_v u @%. t')
+  | S16, S32 -> int16_to_int32 u
+  | S16, S64 -> int16_to_int64 u
+  | S16, S128 -> pow2_le_compat (bits t' - 1) (bits t - 1); mk_int #S128 #l' (v u)
   
+  | S32, U1 -> UInt8.rem (int32_to_uint8 u) 2uy
+  | S32, U8 -> int32_to_uint8 u
+  | S32, U16 -> int32_to_uint16 u
+  | S32, U32 -> int32_to_uint32 u
+  | S32, U64 -> int32_to_uint64 u
+  | S32, U128 -> pow2_le_compat (bits t') (bits t - 1); mk_int #U128 #l' (v u % modulus U128)
+  | S32, S8 -> int32_to_int8 u
+  | S32, S16 -> int32_to_int16 u
+  | S32, S32 -> u
+  | S32, S64 -> int32_to_int64 u
+  | S32, S128 -> pow2_le_compat (bits t' - 1) (bits t - 1); mk_int #S128 #l' (v u)
+
+  | S64, U1 -> UInt8.rem (int64_to_uint8 u) 2uy
+  | S64, U8 -> int64_to_uint8 u
+  | S64, U16 -> int64_to_uint16 u
+  | S64, U32 -> int64_to_uint32 u
+  | S64, U64 -> int64_to_uint64 u
+  | S64, U128 -> pow2_le_compat (bits t') (bits t - 1); mk_int #U128 #l' (v u % modulus U128)
+  | S64, S8 -> int64_to_int8 u
+  | S64, S16 -> int64_to_int16 u
+  | S64, S32 -> int64_to_int32 u
+  | S64, S64 -> u
+  | S64, S128 -> pow2_le_compat (bits t' - 1) (bits t - 1); mk_int #S128 #l' (v u)
+  
+  | S128, S128 -> u
+  | S128, _ -> mk_int #t' #l' (v u @%. t')
+
+#pop-options
+
+let ones t l = mk_int #t #l (ones_v t)
+
+let zeros t l = mk_int 0
 
 let add_mod #t #l a b =
   match t with
@@ -268,10 +249,10 @@ let add_mod #t #l a b =
   | U32  -> UInt32.add_mod a b
   | U64  -> UInt64.add_mod a b
   | U128 -> UInt128.add_mod a b
-  | S8 -> Int8.int_to_t (Int.add_mod (Int8.v a) (Int8.v b))
-  | S16 -> Int16.int_to_t (Int.add_mod (Int16.v a) (Int16.v b))
-  | S32 -> Int32.int_to_t (Int.add_mod (Int32.v a) (Int32.v b))
-  | S64 -> Int64.int_to_t (Int.add_mod (Int64.v a) (Int64.v b))
+  | S8   -> Int8.int_to_t (Int.add_mod (Int8.v a) (Int8.v b))
+  | S16  -> Int16.int_to_t (Int.add_mod (Int16.v a) (Int16.v b))
+  | S32  -> Int32.int_to_t (Int.add_mod (Int32.v a) (Int32.v b))
+  | S64  -> Int64.int_to_t (Int.add_mod (Int64.v a) (Int64.v b))
   | S128 -> Int128.int_to_t (Int.add_mod (Int128.v a) (Int128.v b))
 
 let add_mod_lemma #t #l a b = ()
@@ -292,6 +273,8 @@ let add #t #l a b =
   
 let add_lemma #t #l a b = ()
 
+#push-options "--max_fuel 1"
+
 let incr #t #l a =
   match t with
   | U1   -> UInt8.add a 0x1uy
@@ -305,8 +288,10 @@ let incr #t #l a =
   | S32 -> Int32.add a 0x1l
   | S64 -> Int64.add a 0x1L
   | S128 -> Int128.add a (Int128.int_to_t 1)
-  
+
 let incr_lemma #t #l a = ()
+
+#pop-options
 
 let mul_mod #t #l a b =
   match t with
@@ -376,6 +361,8 @@ let sub #t #l a b =
   
 let sub_lemma #t #l a b = ()
 
+#push-options "--max_fuel 1"
+
 let decr #t #l a =
   match t with
   | U1   -> UInt8.sub a 0x1uy
@@ -384,15 +371,15 @@ let decr #t #l a =
   | U32  -> UInt32.sub a 0x1ul
   | U64  -> UInt64.sub a 0x1uL
   | U128 -> UInt128.sub a (UInt128.uint_to_t 1)
-  | S8 -> Int8.sub a 0x1y
-  | S16 -> Int16.sub a 0x1s
-  | S32 -> Int32.sub a 0x1l
-  | S64 -> Int64.sub a 0x1L
+  | S8   -> Int8.sub a 0x1y
+  | S16  -> Int16.sub a 0x1s
+  | S32  -> Int32.sub a 0x1l
+  | S64  -> Int64.sub a 0x1L
   | S128 -> Int128.sub a (Int128.int_to_t 1)
 
 let decr_lemma #t #l a = ()
- 
-#reset-options "--z3rlimit 300"
+
+#pop-options
 
 let logxor #t #l a b =
   match t with
@@ -407,57 +394,57 @@ let logxor #t #l a b =
   | U32  -> UInt32.logxor a b
   | U64  -> UInt64.logxor a b
   | U128 -> UInt128.logxor a b
-  | S8 -> Int8.logxor a b
-  | S16 -> Int16.logxor a b
-  | S32 -> Int32.logxor a b
-  | S64 -> Int64.logxor a b
+  | S8   -> Int8.logxor a b
+  | S16  -> Int16.logxor a b
+  | S32  -> Int32.logxor a b
+  | S64  -> Int64.logxor a b
   | S128 -> Int128.logxor a b
   
-#set-options "--max_fuel 1" 
+#push-options "--max_fuel 1" 
 
 val logxor_lemma_: #t:inttype -> #l:secrecy_level -> a:int_t t l -> b:int_t t l -> Lemma
-  (int_v (a `logxor` (a `logxor` b)) == int_v b)
+  (v (a `logxor` (a `logxor` b)) == v b)
 let logxor_lemma_ #t #l a b =
   match t with
-  |U1 |U8 |U16 |U32 |U64 |U128 ->
-  UInt.logxor_associative #(bits t) (uint_v a) (uint_v a) (uint_v b);
-  UInt.logxor_self #(bits t) (uint_v a);
-  UInt.logxor_commutative #(bits t) 0 (uint_v b);
-  UInt.logxor_lemma_1 #(bits t) (uint_v b)
-  |S8 |S16 |S32 |S64 |S128 ->
-  Int.logxor_associative #(bits t) (sint_v a) (sint_v a) (sint_v b);
-  Int.logxor_self #(bits t) (sint_v a);
-  Int.logxor_commutative #(bits t) 0 (sint_v b);
-  Int.logxor_lemma_1 #(bits t) (sint_v b)
+  | U1 |U8 |U16 |U32 |U64 |U128 ->
+  UInt.logxor_associative #(bits t) (v a) (v a) (v b);
+  UInt.logxor_self #(bits t) (v a);
+  UInt.logxor_commutative #(bits t) 0 (v b);
+  UInt.logxor_lemma_1 #(bits t) (v b)
+  | S8 |S16 |S32 |S64 |S128 ->
+  Int.logxor_associative #(bits t) (v a) (v a) (v b);
+  Int.logxor_self #(bits t) (v a);
+  Int.logxor_commutative #(bits t) 0 (v b);
+  Int.logxor_lemma_1 #(bits t) (v b)
 
 let logxor_lemma #t #l a b =
   logxor_lemma_ #t a b;
-  intv_extensionality (logxor a (logxor a b)) b;
+  v_extensionality (logxor a (logxor a b)) b;
   assert (a `logxor` (a `logxor` b) == b);
   (match t with |U1 |U8 |U16 |U32 |U64 |U128 ->
-   UInt.logxor_commutative #(bits t) (uint_v a) (uint_v b)
-   |S8 |S16 |S32 |S64 |S128 -> Int.logxor_commutative #(bits t) (sint_v a) (sint_v b));
+   UInt.logxor_commutative #(bits t) (v a) (v b)
+   |S8 |S16 |S32 |S64 |S128 -> Int.logxor_commutative #(bits t) (v a) (v b));
   logxor_lemma_ #t a b;
-  intv_extensionality (logxor a (logxor b a)) b;
+  v_extensionality (logxor a (logxor b a)) b;
   assert ((a `logxor` (b `logxor` a)) == b);
   (match t with |U1 |U8 |U16 |U32 |U64 |U128 ->
-   UInt.logxor_lemma_1 #(bits t) (uint_v a)
-   |S8 |S16 |S32 |S64 |S128 -> Int.logxor_lemma_1 #(bits t) (sint_v a));
-  //UInt.logxor_lemma_1 #(bits t) (uint_v a);
-  intv_extensionality (logxor a (mk_int #t #l 0)) a
+   UInt.logxor_lemma_1 #(bits t) (v a)
+   |S8 |S16 |S32 |S64 |S128 -> Int.logxor_lemma_1 #(bits t) (v a));
+  //UInt.logxor_lemma_1 #(bits t) (v a);
+  v_extensionality (logxor a (mk_int #t #l 0)) a
 
 let logxor_lemma1 #t #l a b =
-  match (v a, v b) with
+  match v a, v b with
   | _, 0 ->
-    UInt.logxor_lemma_1 #(bits t) (int_v a)
+    UInt.logxor_lemma_1 #(bits t) (v a)
   | 0, _ ->
-    UInt.logxor_commutative #(bits t) (int_v a) (int_v b);
-    UInt.logxor_lemma_1 #(bits t) (int_v b)
+    UInt.logxor_commutative #(bits t) (v a) (v b);
+    UInt.logxor_lemma_1 #(bits t) (v b)
   | 1, 1 ->
-    intv_extensionality a b;
-    UInt.logxor_self #(bits t) (int_v a)
+    v_extensionality a b;
+    UInt.logxor_self #(bits t) (v a)
 
-#set-options "--max_fuel 0"
+#pop-options
 
 let logand #t #l a b =
   match t with
@@ -478,24 +465,15 @@ let logand #t #l a b =
   | S64 -> Int64.logand a b
   | S128 -> Int128.logand a b
 
-let logand_lemma #t a b =
+let logand_zeros #t #l a =
   match t with 
-  |U8 |U16 |U32 |U64 |U128 ->
-   if (uint_v a = 0) then begin
-    UInt.logand_commutative #(bits t) (uint_v a) (uint_v b);
-    UInt.logand_lemma_1 #(bits t) (uint_v b) end
-  else begin
-    UInt.logand_commutative #(bits t) (uint_v a) (uint_v b);
-    UInt.logand_lemma_2 #(bits t) (uint_v b) end
-  |S8 |S16 |S32 |S64 | S128 ->
-   if (sint_v a = 0) then begin
-    Int.logand_commutative #(bits t) (sint_v a) (sint_v b);
-    Int.logand_lemma_1 #(bits t) (sint_v b) end
-  else begin
-    Int.logand_commutative #(bits t) (sint_v a) (sint_v b);
-    Int.logand_lemma_2 #(bits t) (sint_v b) end
+  | U8 | U16 | U32 | U64 | U128 -> UInt.logand_lemma_1 #(bits t) (v a)
+  | S8 | S16 | S32 | S64 | S128 -> Int.logand_lemma_1 #(bits t) (v a)
 
-#reset-options "--z3rlimit 300"
+let logand_ones #t #l a =
+  match t with 
+  | U8 | U16 | U32 | U64 | U128 -> UInt.logand_lemma_2 #(bits t) (v a)
+  | S8 | S16 | S32 | S64 | S128 -> Int.logand_lemma_2 #(bits t) (v a)
 
 let logand_spec #t #l a b = ()
 
@@ -512,26 +490,29 @@ let logor #t #l a b =
   | U32  -> UInt32.logor a b
   | U64  -> UInt64.logor a b
   | U128 -> UInt128.logor a b
-  | S8 -> Int8.logor a b
-  | S16 -> Int16.logor a b
-  | S32 -> Int32.logor a b
-  | S64 -> Int64.logor a b
+  | S8   -> Int8.logor a b
+  | S16  -> Int16.logor a b
+  | S32  -> Int32.logor a b
+  | S64  -> Int64.logor a b
   | S128 -> Int128.logor a b
   
 let logor_spec #t #l a b = ()
 
-#set-options "--max_fuel 1"
+#push-options "--max_fuel 1"
 
-let logor_disjoint #t a b m =
-  if m > 0 then begin
-    UInt.logor_disjoint #(bits t) (uint_v b) (uint_v a) m;
-    UInt.logor_commutative #(bits t) (uint_v b) (uint_v a) end
-  else begin
-    UInt.logor_commutative #(bits t) (uint_v a) (uint_v b);
-    UInt.logor_lemma_1 #(bits t) (uint_v b)
+let logor_disjoint #t #l a b m =
+  if m > 0 then 
+  begin
+    UInt.logor_disjoint #(bits t) (v b) (v a) m;
+    UInt.logor_commutative #(bits t) (v b) (v a)
   end
-    
-#set-options "--max_fuel 0"
+  else 
+  begin
+    UInt.logor_commutative #(bits t) (v a) (v b);
+    UInt.logor_lemma_1 #(bits t) (v b)
+  end
+  
+#pop-options
 
 let lognot #t #l a =
   match t with
@@ -541,15 +522,15 @@ let lognot #t #l a =
   | U32  -> UInt32.lognot a
   | U64  -> UInt64.lognot a
   | U128 -> UInt128.lognot a
-  | S8 -> Int8.lognot a
-  | S16 -> Int16.lognot a
-  | S32 -> Int32.lognot a
-  | S64 -> Int64.lognot a
+  | S8   -> Int8.lognot a
+  | S16  -> Int16.lognot a
+  | S32  -> Int32.lognot a
+  | S64  -> Int64.lognot a
   | S128 -> Int128.lognot a
   
 let shift_right_negative (#n:pos) (a:Int.int_t n{a < 0}) (s:nat) : Tot (Int.int_t n) =
   let shift_right_negative_vec (#n:pos) (a:BitVector.bv_t n) (s:nat) : Tot (BitVector.bv_t n) =
-  if s>= n then BitVector.ones_vec #n
+  if s >= n then BitVector.ones_vec #n
   else if s = 0 then a
   else Seq.append (BitVector.ones_vec #s) (Seq.slice a 0 (n-s))
   in FStar.Int.from_vec (shift_right_negative_vec #n (FStar.Int.to_vec #n a) s)
@@ -568,14 +549,11 @@ let shift_right #t #l a b =
   | S64 -> Int64.shift_arithmetic_right a b
   | S128 -> Int128.shift_arithmetic_right a b
 
-#reset-options "--z3rlimit 500 --max_fuel 2 --max_ifuel 2"
-
 val shift_right_value_aux_1: #n:pos{n>1} -> a:Int.int_t n -> s:nat{s >= n} ->
-  Lemma (requires True)
-        (ensures Int.shift_arithmetic_right #n a s = a / pow2 s)
+  Lemma (Int.shift_arithmetic_right #n a s = a / pow2 s)
 let shift_right_value_aux_1 #n a s =
   pow2_le_compat s n;
-  if (a>=0) then (Int.sign_bit_positive a; assert(a=Int.to_uint a); assert(Int.shift_arithmetic_right #n a s == UInt.shift_right #n a s); UInt.shift_right_value_aux_1 #n a s)
+  if a >= 0 then (Int.sign_bit_positive a; assert(a=Int.to_uint a); assert(Int.shift_arithmetic_right #n a s == UInt.shift_right #n a s); UInt.shift_right_value_aux_1 #n a s)
   else begin
   Int.sign_bit_negative a;
   assert (Int.shift_arithmetic_right #n a s = -1);
@@ -586,11 +564,8 @@ let shift_right_value_aux_1 #n a s =
   end
   
 val shift_right_value_aux_2: #n:pos -> a:Int.int_t n ->
-  Lemma (requires True)
-        (ensures Int.shift_arithmetic_right #n a 0 = a / pow2 0)
+  Lemma (Int.shift_arithmetic_right #n a 0 = a / pow2 0)
 let shift_right_value_aux_2 #n a = assert_norm (pow2 0 == 1)
-
-#reset-options "--z3rlimit 500 --max_fuel 2 --max_ifuel 2"
 
 // val append_lemma: #n:pos -> #m:pos -> a:BitVector.bv_t n -> b:BitVector.bv_t m ->
 //   Lemma (Int.from_vec #(n + m) (Seq.append a b) = (Int.from_vec #n a) * pow2 m + (UInt.from_vec #m b))
@@ -634,9 +609,6 @@ let shift_right_value_aux_0 #n a =
   assert (sar = a / 2)
   end
 
-
-#reset-options "--z3rlimit 500 --max_fuel 2 --max_ifuel 2"
-
 val shift_right_value_aux_3: #n:pos -> a:Int.int_t n -> s:pos{s < n} ->
   Lemma (requires True)
         (ensures Int.shift_arithmetic_right #n a s = a / pow2 s)
@@ -658,9 +630,9 @@ let rec shift_right_value_aux_3 #n a s =
 let shift_right_lemma #t #l a b = 
   match t with
   |U1 |U8 |U16 |U32 |U64 |U128 -> ()
-  |S8 |S16 |S32 |S64 |S128 -> if (int_v b >= bits t) then shift_right_value_aux_1 #(bits t) (int_v a) (int_v b)
-       else if (int_v b = 0) then shift_right_value_aux_2 #(bits t) (int_v a)
-       else shift_right_value_aux_3 #(bits t) (int_v a) (int_v b)
+  |S8 |S16 |S32 |S64 |S128 -> if (v b >= bits t) then shift_right_value_aux_1 #(bits t) (v a) (v b)
+       else if (v b = 0) then shift_right_value_aux_2 #(bits t) (v a)
+       else shift_right_value_aux_3 #(bits t) (v a) (v b)
   
 let shift_left_negative (#n:pos) (a:Int.int_t n{a < 0}) (s:nat) : Tot (Int.int_t n) =
   FStar.Int.from_vec (BitVector.shift_left_vec #n (FStar.Int.to_vec #n a) s)
@@ -673,24 +645,24 @@ let shift_left #t #l a b =
   | U32  -> UInt32.shift_left a b
   | U64  -> UInt64.shift_left a b
   | U128 -> UInt128.shift_left a b
-  | S8 -> if (sint_v a >= 0) then Int8.shift_left a b
+  | S8 -> if (v a >= 0) then Int8.shift_left a b
          else Int8.int_to_t (shift_left_negative (Int8.v a) (UInt32.v b))
-  | S16 -> if (sint_v a >= 0) then Int16.shift_left a b
+  | S16 -> if (v a >= 0) then Int16.shift_left a b
          else Int16.int_to_t (shift_left_negative (Int16.v a) (UInt32.v b))
-  | S32 -> if (sint_v a >= 0) then Int32.shift_left a b
+  | S32 -> if (v a >= 0) then Int32.shift_left a b
          else Int32.int_to_t (shift_left_negative (Int32.v a) (UInt32.v b))
-  | S64 -> if (sint_v a >= 0) then Int64.shift_left a b
+  | S64 -> if (v a >= 0) then Int64.shift_left a b
          else Int64.int_to_t (shift_left_negative (Int64.v a) (UInt32.v b))
-  | S128 -> if (sint_v a >= 0) then Int128.shift_left a b
+  | S128 -> if (v a >= 0) then Int128.shift_left a b
          else Int128.int_to_t (shift_left_negative (Int128.v a) (UInt32.v b))
-         
-#reset-options "--z3rlimit 800 --max_fuel 3 --max_ifuel 3"
+
+#push-options "--max_fuel 1"
 
 let shift_left_lemma #t #l a b = 
   match t with
   |U1 |U8 |U16 |U32 |U64 |U128 -> ()
-  |_ -> let a' = int_v a in
-       let b' = int_v b in
+  |_ -> let a' = v a in
+       let b' = v b in
        let n = Int.to_uint a' in
        let sn = UInt.shift_left #(bits t) n b' in
        assert(Int.to_vec a' == UInt.to_vec #(bits t) n); 
@@ -708,31 +680,17 @@ let shift_left_lemma #t #l a b =
        assert (sn == (a' * pow2 b') % pow2 (bits t));
        ())
 
-
 let rotate_right #t #l a b =
   logor (shift_right a b) (shift_left a (sub #U32 (size (bits t)) b))
 
 let rotate_left #t #l a b =
   logor (shift_left a b) (shift_right a (sub #U32 (size (bits t)) b))
 
-let zeroes t l = nat_to_int #t #l 0
-
-let ones t l =
-  match t with
-  | U1  -> 0x1uy
-  | U8  -> 0xFFuy
-  | U16 -> 0xFFFFus
-  | U32 -> 0xFFFFFFFFul
-  | U64 -> 0xFFFFFFFFFFFFFFFFuL
-  | U128 ->
-    let x = UInt128.uint64_to_uint128 0xFFFFFFFFFFFFFFFFuL in
-    let y = (UInt128.shift_left x 64ul) `UInt128.add` x in
-    assert_norm (UInt128.v y == pow2 128 - 1);
-    y
-  | _  -> mk_int #t #l (ones_v t)
-
 inline_for_extraction
-let minus (#t:inttype) (#l:secrecy_level) (a:int_t t l) = add_mod (lognot a) (mk_int #t #l 1)
+let minus (#t:inttype) (#l:secrecy_level) (a:int_t t l) = 
+  add_mod (lognot a) (mk_int #t #l 1)
+
+#pop-options
 
 let eq_mask #t a b =
   match t with
@@ -748,7 +706,7 @@ let eq_mask #t a b =
   | S64  -> to_i64 (UInt64.eq_mask (to_u64 a) (to_u64 b))
   | S128 -> to_i128 (UInt128.eq_mask (to_u128 a) (to_u128 b))
 
-#reset-options "--z3rlimit 3000 --max_fuel 1 --max_ifuel 1"
+let op_At_Percent = Int.op_At_Percent
 
 let eq_mask_lemma #t a b =
   match t with
@@ -824,13 +782,19 @@ let eq_mask_lemma #t a b =
 
 let eq_mask_logand_lemma #t a b c =
   eq_mask_lemma a b;
-  logand_lemma (eq_mask a b) c;
+  logand_zeros c;
+  logand_ones c;
   match t with 
-  | U8 | U16 | U32 | U64 | U128 -> UInt.logand_commutative #(bits t) (uint_v (eq_mask a b)) (uint_v c)
-  | _ -> Int.logand_commutative #(bits t) (uint_v (eq_mask a b)) (uint_v c)
+  | U8 | U16 | U32 | U64 | U128 -> UInt.logand_commutative #(bits t) (v (eq_mask a b)) (v c)
   
 let neq_mask #t a b = lognot (eq_mask #t a b)
 
+let neq_mask_lemma #t a b = 
+  match t with
+  | U8 | U16 | U32 | U64 | U128 -> 
+    UInt.lognot_lemma_1 #(bits t);
+    UInt.lognot_self #(bits t) 0
+  
 let gte_mask #t a b =
   match t with
   | U1   -> logor a (lognot b)
@@ -852,56 +816,65 @@ let gte_mask_lemma #t a b =
   | _ -> ()
 
 let gte_mask_logand_lemma #t a b c =
-  gte_mask_lemma a b;
-  logand_lemma (gte_mask a b) c;
-  UInt.logand_commutative #(bits t) (uint_v (gte_mask a b)) (uint_v c)
+  logand_zeros c;
+  logand_ones c;
+  UInt.logand_commutative #(bits t) (v (gte_mask a b)) (v c)
 
 let lt_mask #t a b = lognot (gte_mask a b)
 
+let lt_mask_lemma #t a b =
+  UInt.lognot_lemma_1 #(bits t);
+  UInt.lognot_self #(bits t) 0
+
 let gt_mask #t a b = logand (gte_mask a b) (neq_mask a b)
+
+let gt_mask_lemma #t a b =
+  logand_zeros (gte_mask a b);
+  logand_ones (gte_mask a b)
 
 let lte_mask #t a b = logor (lt_mask a b) (eq_mask a b)
 
-#reset-options "--z3rlimit 3000 --max_fuel 3 --max_ifuel 3"
-
-private
+let lte_mask_lemma #t a b =
+  match t with 
+  | U8 | U16 | U32 | U64 | U128 ->
+    assume (v a > v b);
+    UInt.logor_lemma_1 #(bits t) (v (lt_mask a b));
+    UInt.logor_lemma_2 #(bits t) (v (eq_mask a b))
+ 
+ private
 val mod_mask_value: #t:inttype -> #l:secrecy_level -> m:shiftval t ->
-  Lemma (int_v (mod_mask #t #l m) == pow2 (uint_v m) - 1)
+  Lemma (v (mod_mask #t #l m) == pow2 (v m) - 1)
+
+#push-options "--max_fuel 1 "
 
 let mod_mask_value #t #l m =
-  shift_left_lemma (nat_to_int #t #l 1) m;
+  shift_left_lemma (mk_int #t #l 1) m;
   pow2_double_mult ((bits t) - 1);
-  pow2_le_compat (uint_v m) 0;
-  pow2_lt_compat (bits t) (uint_v m);
-  small_modulo_lemma_1 (pow2 (uint_v m)) (pow2 (bits t));
-  small_modulo_lemma_1 ((pow2 (uint_v m)) -1) (pow2 (bits t));
-  assert( int_v (mod_mask #t #l m) == (((1 * pow2 (uint_v m)) @%. t) - 1) @%. t);
+  pow2_le_compat (v m) 0;
+  pow2_lt_compat (bits t) (v m);
+  small_modulo_lemma_1 (pow2 (v m)) (pow2 (bits t));
+  small_modulo_lemma_1 ((pow2 (v m)) -1) (pow2 (bits t));
+  assert(v (mod_mask #t #l m) == (((1 * pow2 (v m)) @%. t) - 1) @%. t);
   match t with
   |U1 |U8 |U16 |U32 |U64 |U128 -> ()
-  |_ -> if (uint_v m < (bits t) -1) then (pow2_lt_compat ((bits t)-1) (uint_v m); assert((1*pow2 (uint_v m))@%. t = pow2 (uint_v m))) else (assert ((1* pow2 (uint_v m)) @%. t = pow2 (uint_v m) - pow2 (bits t)); assert (uint_v m = (bits t) -1); pow2_double_mult ((bits t) -1); assert ((1 * pow2 (uint_v m)) @%. t = - pow2 (uint_v m))) 
-
-#set-options "--max_fuel 1"
+  |_ -> if (v m < (bits t) -1) then (pow2_lt_compat (bits t - 1) (v m); assert((1*pow2 (v m))@%. t = pow2 (v m))) else (assert ((1* pow2 (v m)) @%. t = pow2 (v m) - pow2 (bits t)); assert (v m = (bits t) -1); pow2_double_mult ((bits t) -1); assert ((1 * pow2 (v m)) @%. t = - pow2 (v m))) 
 
 let mod_mask_lemma #t #l a m =
   mod_mask_value #t #l m;
   match t with
   |U1 |U8 |U16 |U32 |U64 |U128 ->
-  if uint_v m = 0 then
-    UInt.logand_lemma_1 #(bits t) (uint_v a)
+  if v m = 0 then
+    UInt.logand_lemma_1 #(bits t) (v a)
   else
-    UInt.logand_mask #(bits t) (uint_v a) (uint_v m) 
+    UInt.logand_mask #(bits t) (v a) (v m) 
   |_->
-  if uint_v m = 0 then
-    Int.logand_lemma_1 #(bits t) (sint_v a)
+  if v m = 0 then
+    Int.logand_lemma_1 #(bits t) (v a)
   else admit() 
-  
-#set-options "--max_fuel 0"
 
-(* defined in .fsti: notations +^, -^, ...*)
+#pop-options
 
 let nat_mod_v #m x = x
-
-#reset-options "--z3rlimit 3000 --max_fuel 1 --max_ifuel 1"
 
 let div #t x y =
   match t with
